

## 【Basic Requirement】

- (1) Derive the closed-form formula using the martingale pricing method by hands.

First we find the payoff function from the diagram, define:

$$f(S_t) := \begin{cases} 0 & \text{if } S_t < K_1 \text{ or } S_t > K_4 \\ S_t - K_1 & \text{if } K_1 \leq S_t < K_2 \\ K_2 - K_1 & \text{if } K_2 \leq S_t < K_3 \\ (K_2 - K_1) - (S_t - K_3) \frac{K_2 - K_1}{K_4 - K_3} & \text{if } K_3 \leq S_t \leq K_4 \end{cases}$$

If we further define:

$$I_A(S_t) = \begin{cases} 1 & \text{if } K_1 \leq S_t < K_2 \\ 0 & \text{otherwise} \end{cases}, I_B(S_t) = \begin{cases} 1 & \text{if } K_2 \leq S_t < K_3 \\ 0 & \text{otherwise} \end{cases}, I_C(S_t) = \begin{cases} 1 & \text{if } K_3 \leq S_t \leq K_4 \\ 0 & \text{otherwise} \end{cases}$$

Then we have:

$$f(S_t) = (S_t - K_1)I_A(S_t) + (K_2 - K_1)I_B(S_t) + \left[ (K_2 - K_1) - (S_t - K_3) \frac{K_2 - K_1}{K_4 - K_3} \right] I_C(S_t)$$

To find the present value of such an option, we must evaluate the expected value of  $f(S_t)$ , i.e.

$E[f(S_t)]$ . By the linearity of expected value, we have:

$$\begin{aligned} E[f(S_t)] &= E[(S_t - K_1)I_A(S_t)] + E[(K_2 - K_1)I_B(S_t)] \\ &\quad + E\left[\left[(K_2 - K_1) - (S_t - K_3) \frac{K_2 - K_1}{K_4 - K_3}\right] I_C(S_t)\right] \\ &= E[S_t I_A(S_t)] - K_1 E[I_A(S_t)] + (K_2 - K_1) E[I_B(S_t)] + (K_2 - K_1) E[I_C(S_t)] \\ &\quad + K_3 \frac{K_2 - K_1}{K_4 - K_3} E[I_C(S_t)] - \frac{K_2 - K_1}{K_4 - K_3} E[S_t I_C(S_t)] \end{aligned}$$

Now, we evaluate each term on the right-hand-side of the equal sign. Since we want to apply

**Girsanov Theorem** on some of the upcoming computation. Let the probability measure we use above be “measure Q”.

Let's start with  $E[S_t I_A(S_t)]$ :

$$\begin{aligned} E[S_t I_A(S_t)] &:= E^Q[S_t I_A(S_t)] = E^Q\left[S_0 \cdot e^{\left(r-q-\frac{\sigma^2}{2}\right)T + \sigma \Delta Z^Q(T)} \cdot I_A(S_T)\right] \\ &= S_0 e^{(r-q)T} \cdot E^Q\left[e^{-\frac{\sigma^2}{2}T + \sigma \Delta Z^Q(T)} \cdot I_A(S_T)\right] \dots (*) \end{aligned}$$

If we setting  $H(t)$  in **Girsanov Theorem** equals to  $H(t) = -\sigma$ , we have:

$$\Lambda = \frac{dR}{dQ} = e^{-\frac{1}{2} \int_0^T \sigma^2 d\tau - \int_0^T -\sigma dZ^Q(\tau)} = e^{-\frac{\sigma^2}{2}T + \sigma \Delta Z^Q(T)}$$

Plug the result above in (\*), we have:

$$\begin{aligned} E^Q[S_t I_A(S_t)] &= S_0 e^{(r-q)T} \cdot E^Q[\Lambda \cdot I_A(S_T)] = S_0 e^{(r-q)T} \cdot E^R[I_A(S_T)] \\ &= S_0 e^{(r-q)T} \cdot \Pr^R(\{K_1 \leq S_t < K_2\}) \end{aligned}$$

After apply nature log function on  $S_t, K$ , replace  $S_t$  with  $\ln S_0 + \left(r - q + \frac{\sigma^2}{2}\right)T + \sigma \Delta Z^R(T)$ ,

and last normalization, we have:

$$\mathbb{E}^Q[S_t I_A(S_t)] = S_0 e^{(r-q)T} \cdot \text{Pr}^R \left( \left\{ -\frac{\Delta Z^R(T)}{\sqrt{T}} \leq \frac{\ln \frac{S_0}{K_1} + \left(r - q + \frac{\sigma^2}{2}\right)T}{\sigma \sqrt{T}} \right\} \setminus \left\{ \frac{\Delta Z^R(T)}{\sqrt{T}} \leq \frac{\ln \frac{S_0}{K_2} + \left(r - q + \frac{\sigma^2}{2}\right)T}{\sigma \sqrt{T}} \right\} \right)$$

Define  $d_{1,R} := \frac{\ln \frac{S_0}{K_1} + \left(r - q + \frac{\sigma^2}{2}\right)T}{\sigma \sqrt{T}}$ ,  $d_{2,R} := \frac{\ln \frac{S_0}{K_2} + \left(r - q + \frac{\sigma^2}{2}\right)T}{\sigma \sqrt{T}}$ , we obtain the result of:

$$\mathbb{E}^Q[S_t I_A(S_t)] = S_0 e^{(r-q)T} \cdot [N(d_{2,R}) - N(d_{1,R})]$$

As for  $\mathbb{E}[I_A(S_t)]$ , there's NO need of applying **Girsanov Theorem**, we simply use the step above,

i.e. nature log, replace  $S_t$  and then normalize, we can obtain:

$$\mathbb{E}[I_A(S_t)] = [N(d_{2,Q}) - N(d_{1,Q})]$$

Where  $d_{1,Q} := \frac{\ln \frac{S_0}{K_1} + \left(r - q - \frac{\sigma^2}{2}\right)T}{\sigma \sqrt{T}}$ ,  $d_{2,Q} := \frac{\ln \frac{S_0}{K_2} + \left(r - q - \frac{\sigma^2}{2}\right)T}{\sigma \sqrt{T}}$

With similar method, and define  $d_{i,Q} := \frac{\ln \frac{S_0}{K_i} + \left(r - q - \frac{\sigma^2}{2}\right)T}{\sigma \sqrt{T}}$ ,  $d_{i,R} := \frac{\ln \frac{S_0}{K_i} + \left(r - q + \frac{\sigma^2}{2}\right)T}{\sigma \sqrt{T}}$  we can also

obtain:

$$\mathbb{E}[I_B(S_t)] = [N(d_{3,Q}) - N(d_{2,Q})]$$

$$\mathbb{E}[I_C(S_t)] = [N(d_{4,Q}) - N(d_{3,Q})]$$

$$\mathbb{E}[S_t I_C(S_t)] = S_0 e^{(r-q)T} \cdot [N(d_{4,R}) - N(d_{3,R})]$$

With these result, we can finally conclude that:

$$\begin{aligned} \mathbb{E}[f(S_t)] &= S_0 e^{(r-q)T} \cdot [N(d_{2,R}) - N(d_{1,R})] - K_1 [N(d_{2,Q}) - N(d_{1,Q})] \\ &\quad + (K_2 - K_1) [N(d_{3,Q}) - N(d_{2,Q})] + (K_2 - K_1) [N(d_{4,Q}) - N(d_{3,Q})] \\ &\quad + K_3 \frac{K_2 - K_1}{K_4 - K_3} [N(d_{4,Q}) - N(d_{3,Q})] - \frac{K_2 - K_1}{K_4 - K_3} S_0 e^{(r-q)T} \cdot [N(d_{4,R}) - N(d_{3,R})] \\ &= S_0 e^{(r-q)T} \cdot [N(d_{2,R}) - N(d_{1,R})] \\ &\quad + K_1 N(d_{1,Q}) - K_2 N(d_{2,Q}) + K_2 N(d_{4,Q}) - K_1 N(d_{4,Q}) \\ &\quad + K_3 \frac{K_2 - K_1}{K_4 - K_3} [N(d_{4,Q}) - N(d_{3,Q})] - \frac{K_2 - K_1}{K_4 - K_3} S_0 e^{(r-q)T} \cdot [N(d_{4,R}) - N(d_{3,R})] \end{aligned}$$

The last step is to discount the expected value with  $r$ , finally we can Derive the closed-form

formula of the value of this derivative

$$e^{-rt} \cdot \mathbb{E}[f(S_t)] =$$

$$\begin{aligned} e^{-rt} \left\{ S_0 e^{(r-q)T} \cdot [N(d_{2,R}) - N(d_{1,R})] + K_1 N(d_{1,Q}) - K_2 N(d_{2,Q}) + K_2 N(d_{4,Q}) - K_1 N(d_{4,Q}) \right. \\ \left. + K_3 \frac{K_2 - K_1}{K_4 - K_3} [N(d_{4,Q}) - N(d_{3,Q})] - \frac{K_2 - K_1}{K_4 - K_3} S_0 e^{(r-q)T} \cdot [N(d_{4,R}) - N(d_{3,R})] \right\} \end{aligned}$$

(2) blahblahblah

(3)